Some material on appending and filtering inputs, some cleanup

Ranking.thy
@@ -10,8 +10,16 @@ sledgehammer_params [provers = e z3 spass cvc4 vampire]
 lemma vs_empty[simp]: "Vs {} = {}"
   by (simp add: Vs_def)
 
+lemma vs_insert: "Vs (insert e E) = e \<union> Vs E"
+  unfolding Vs_def by simp
+
 lemma vs_union: "Vs (A \<union> B) = Vs A \<union> Vs B"
   unfolding Vs_def by simp
+
+lemma vs_compr: "Vs {{u, v} |v. v \<in> ns} = (if ns = {} then {} else {u} \<union> ns)"
+  unfolding Vs_def by auto
+
+
 
 lemma graph_abs_empty[simp]: "graph_abs {}"
   by (simp add: graph_abs_def)
@@ -46,6 +54,7 @@ lemma partitioned_bipartite_graph_absD:
   unfolding partitioned_bipartite_def
   by (auto intro: graph_abs.intro)
 
+
 lemma partitioned_bipartiteE:
   assumes "partitioned_bipartite E X"
   assumes "e \<in> E"
@@ -54,11 +63,37 @@ lemma partitioned_bipartiteE:
   unfolding partitioned_bipartite_def
   by fast
 
+lemma partitioned_bipartite_insertI:
+  assumes "partitioned_bipartite E X"
+  assumes "u \<notin> X" "v \<in> X"
+  shows "partitioned_bipartite (insert {u,v} E) X"
+  using assms
+  apply (intro partitioned_bipartiteI)
+   apply (drule partitioned_bipartite_graph_absD)
+  by (auto simp: vs_insert elim!: partitioned_bipartiteE intro: graph_abs_insert dest: partitioned_bipartite_graph_absD)
+
+lemma partitioned_bipartite_union:
+  assumes "partitioned_bipartite G X"
+  assumes "partitioned_bipartite H X"
+  shows "partitioned_bipartite (G \<union> H) X"
+  using assms partitioned_bipartite_graph_absD
+  by (auto intro!: partitioned_bipartiteI intro: graph_abs_union simp: vs_union)
+     (meson DiffD1 DiffD2 partitioned_bipartiteE)+
+
+lemma partitioned_bipartite_compr:
+  assumes "u \<notin> X" "u \<notin> Y" "finite X" "X \<subseteq> Y"
+  shows "partitioned_bipartite {{u,v} |v. v \<in> X} Y"
+  using assms
+  by (intro partitioned_bipartiteI)
+     (auto simp: graph_abs_compr vs_compr)
+  
+
 type_synonym 'a graph = "'a set set"
 
-text \<open>For now we don't care about distinctness of the "ranking" list, as we only need the order
-  induced by the list.\<close>
+
 abbreviation "rank \<sigma> v \<equiv> index \<sigma> v"
+abbreviation "arrival \<equiv> index \<circ> map fst"
+
 
 lemma index_Cons_mono: "x \<noteq> y \<Longrightarrow> index xs y \<le> index (x#xs) y"
   by simp
@@ -66,8 +101,9 @@ lemma index_Cons_mono: "x \<noteq> y \<Longrightarrow> index xs y \<le> index (x
 lemma index_filter_mono: "P x \<Longrightarrow> index (filter P xs) x \<le> index xs x"
   by (induction xs) auto
 
-lemma index_append_mono: "index xs x \<le> index (xs @ ys) x"
-  by (induction xs) auto
+lemma index_append_mono: "index xs x \<le> index (xs @ ys) x" 
+  unfolding index_def
+  by (auto simp: find_index_append find_index_le_size trans_le_add1)
 
 abbreviation "arriving_U us \<equiv> fst ` set us"
 abbreviation "arriving_V us \<equiv> \<Union> (snd ` set us)"
@@ -78,6 +114,12 @@ definition wf_input :: "'a list \<Rightarrow> ('a \<times> 'a set) list \<Righta
     arriving_V us \<subseteq> set \<sigma> \<and>
     distinct \<sigma> \<and> 
     distinct (map fst us)"
+
+lemma wf_input_distinctD:
+  assumes "wf_input \<sigma> us"
+  shows "distinct \<sigma>"
+  using assms
+  unfolding wf_input_def by auto
 
 fun neighbors_of :: "'a \<Rightarrow> ('a \<times> 'a set) list \<Rightarrow> 'a set" where
   "neighbors_of _ [] = {}"
@@ -103,15 +145,31 @@ fun ranking_aux :: "'a list \<Rightarrow> ('a \<times> 'a set) list \<Rightarrow
   "ranking_aux _ [] M = M"
 | "ranking_aux \<sigma> ((u,ns)#us) M = ranking_aux \<sigma> us (step \<sigma> M u ns)"
 
+lemma ranking_aux_is_foldl:
+  "ranking_aux \<sigma> us M = foldl (\<lambda>M' (u,ns). step \<sigma> M' u ns) M us"
+  by (induction \<sigma> us M rule: ranking_aux.induct) (auto)
+
+lemma ranking_aux_append_us:
+  "ranking_aux \<sigma> (us@us') M = ranking_aux \<sigma> us' (ranking_aux \<sigma> us M)"
+  by (simp add: ranking_aux_is_foldl)
+
 definition ranking :: "'a list \<Rightarrow> ('a \<times> 'a set) list \<Rightarrow> 'a graph" where
   "ranking \<sigma> us = ranking_aux \<sigma> us {}"
+
+lemma ranking_is_foldl:
+  "ranking \<sigma> us = foldl (\<lambda>M (u,ns). step \<sigma> M u ns) {} us"
+  by (simp add: ranking_def ranking_aux_is_foldl)
+
+lemma ranking_append_us:
+  "ranking \<sigma> (us@us') = ranking_aux \<sigma> us' (ranking \<sigma> us)"
+  by (simp add: ranking_aux_append_us ranking_def)
 
 lemma ranking_PI: "P (ranking_aux \<sigma> us {}) \<Longrightarrow> P (ranking \<sigma> us)"
   unfolding ranking_def .
 
 text \<open>The following invariant is maintained by the (steps of the) ranking algorithm.\<close>
 \<comment> \<open>TODO: reconsider the wellformedness of the input in the invariant. It was put there, since the
-  the invariant is only preserved under (some conditions of) wellformedness.\<close>
+   invariant is only preserved under (some conditions of) wellformedness.\<close>
 definition ranking_inv :: "'a list \<Rightarrow> ('a \<times> 'a set) list \<Rightarrow> 'a graph \<Rightarrow> bool" where
   "ranking_inv \<sigma> us M \<equiv> wf_input \<sigma> us \<and> matching M \<and> partitioned_bipartite M (set \<sigma>) \<and> 
     Vs M - set \<sigma> \<subseteq> arriving_U us"
@@ -145,11 +203,20 @@ fun offline_graph :: "('a \<times> 'a set) list \<Rightarrow> 'a graph" where
 lemma step_mono: "e \<in> M \<Longrightarrow> e \<in> step \<sigma> M u ns"
   by (induction \<sigma>) auto
 
+lemma step_mono_Vs: "v \<in> Vs M \<Longrightarrow> v \<in> Vs (step \<sigma> M u ns)"
+  by (auto intro: vs_transport dest: step_mono)
+
 lemma ranking_aux_mono: "e \<in> M \<Longrightarrow> e \<in> ranking_aux \<sigma> us M"
   by (induction \<sigma> us M rule: ranking_aux.induct) (auto simp: step_mono)
 
+lemma ranking_aux_mono_Vs: "v \<in> Vs M \<Longrightarrow> v \<in> Vs (ranking_aux \<sigma> us M)"
+  by (auto intro: vs_transport dest: ranking_aux_mono)
+
 lemma step_empty_if_no_neighbor: "set \<sigma> \<inter> ns = {} \<longleftrightarrow> step \<sigma> {} u ns = {}"
   by (induction \<sigma>) (auto simp: vs_member)
+
+lemma step_no_neighbor: "set \<sigma> \<inter> ns = {} \<Longrightarrow> step \<sigma> M u ns = M"
+  by (induction \<sigma>) auto
 
 lemma wf_input_arriving_disjoint: "wf_input \<sigma> us \<Longrightarrow> arriving_V us \<inter> arriving_U us = {}"
   unfolding wf_input_def by auto
@@ -166,19 +233,33 @@ lemma wf_input_hd': "wf_input \<sigma> (u#us) \<Longrightarrow> fst u \<notin> s
 
 lemma edge_in_step:
   assumes "e \<in> step \<sigma> M u ns"
-  shows "e \<in> M \<or> (\<exists>v.  e = {u,v} \<and> (v \<in> ns \<inter> set \<sigma> - Vs M))"
+  shows "e \<in> M \<or> (\<exists>v. e = {u,v} \<and> (v \<in> ns \<inter> set \<sigma> - Vs M) \<and> (\<forall>v'\<in>ns \<inter> set \<sigma> - Vs M - {v}. rank \<sigma> v < rank \<sigma> v'))"
   using assms
-  by (induction \<sigma> M u ns rule: step.induct) (auto split: if_splits)
+  by (induction \<sigma> M u ns rule: step.induct) 
+     (auto split: if_splits)
+
+lemma edge_in_stepE:
+  assumes "e \<in> step \<sigma> M u ns"
+  assumes "e \<notin> M"
+  obtains v where "e = {u,v}" "v \<in> ns \<inter> set \<sigma> - Vs M" "\<forall>v'\<in> ns \<inter> set \<sigma> - Vs M - {v}. rank \<sigma> v < rank \<sigma> v'"
+  using assms
+  by (auto dest: edge_in_step)
+
 
 lemma edge_in_ranking_aux:
   assumes "e \<in> ranking_aux \<sigma> us M"
-  shows "e \<in> M \<or> (\<exists>u ns v. (u,ns) \<in> set us \<and> v \<in> ns \<and> e = {u,v} \<and> v \<notin> Vs M)"
+  shows "e \<in> M \<or> (\<exists>u ns v. (u,ns) \<in> set us \<and> e = {u,v} \<and> v \<in> ns \<inter> set \<sigma> - Vs M)" \<comment> \<open>The property on v not being in \<^term>\<open>Vs M\<close> is probably not strong enough to be useful.\<close>
   using assms
-  apply (induction \<sigma> us M rule: ranking_aux.induct)
-   apply simp_all
-  apply (erule disjE)
-   apply (drule edge_in_step, blast)
-  by (metis step_mono vs_member)
+  by (induction \<sigma> us M rule: ranking_aux.induct)
+     (auto dest!: edge_in_step step_mono_Vs)
+
+lemma edge_in_ranking_auxE:
+  assumes "e \<in> ranking_aux \<sigma> us M"
+  assumes "e \<notin> M"
+  obtains u ns v where "(u,ns) \<in> set us" "e = {u,v}" "v \<in> ns \<inter> set \<sigma> - Vs M"
+  using assms
+  by (auto dest: edge_in_ranking_aux)
+
 
 lemma vs_step: "v \<in> Vs (step \<sigma> M u ns) \<Longrightarrow> v = u \<or> v \<in> set \<sigma> \<or> v \<in> Vs M"
   by (induction \<sigma> M u ns rule: step.induct) (auto split: if_splits simp: Vs_def)
@@ -196,8 +277,6 @@ qed simp
 lemma vs_offline_graph: "v \<in> Vs (offline_graph us) \<Longrightarrow> v \<in> arriving_U us \<or> v \<in> arriving_V us"
   by (induction us rule: offline_graph.induct) (auto simp: Vs_def)
 
-lemma vs_compr: "Vs {{u, v} |v. v \<in> ns} = (if ns = {} then {} else {u} \<union> ns)"
-  unfolding Vs_def by auto
 
 lemma graph_abs_step:
   assumes "graph_abs M"
@@ -220,17 +299,20 @@ lemma partitioned_bipartite_step:
   shows "partitioned_bipartite (step \<sigma> M u ns) (set \<sigma>)"
   using assms
 proof (induction \<sigma>)
-  case (Cons a \<sigma>)
+  case (Cons v \<sigma>)
   then have graph_abs: "graph_abs (step \<sigma> M u ns)"
     by (auto dest: partitioned_bipartite_graph_absD intro: graph_abs_step)
   show ?case
-    apply (rule step_ConsI)
-    apply (rule partitioned_bipartiteI)
-      apply (metis Cons.prems(2) assms(1) graph_abs_insert list.set_intros(1) partitioned_bipartite_graph_absD)
-     apply (smt (verit, del_insts) Cons.prems(1) Cons.prems(2) Diff_iff edges_are_Vs insert_commute insert_iff list.set(2) partitioned_bipartiteE)
-    apply (rule partitioned_bipartiteI)
-     apply (rule graph_abs)
-    by (smt (verit, del_insts) Cons.prems(1) Cons.prems(2) Diff_iff IntE edge_in_step edges_are_Vs insertCI insert_commute list.set(2) partitioned_bipartiteE)
+  proof (rule step_ConsI)
+    assume "v \<in> ns" "v \<notin> Vs M"
+    with Cons.prems show "partitioned_bipartite (insert {u,v} M) (set (v#\<sigma>))"
+      by (auto intro: partitioned_bipartite_insertI)
+  next
+    assume "v \<notin> ns \<or> v \<in> Vs M"
+    then show "partitioned_bipartite (step \<sigma> M u ns) (set (v#\<sigma>))"
+      by (intro partitioned_bipartiteI[OF graph_abs])
+         (smt (verit, del_insts) Cons.prems(1) Cons.prems(2) Diff_iff IntE edge_in_step edges_are_Vs insertCI insert_commute list.set(2) partitioned_bipartiteE)
+  qed
 qed simp
 
 lemma ranking_inv_step:
@@ -244,40 +326,41 @@ lemma ranking_inv_step:
   by (metis (no_types, lifting) DiffI UnE insert_absorb singleton_insert_inj_eq subset_iff vs_step)
 
 
-lemma wf_input_graph_abs_ranking_aux:
+lemma graph_abs_ranking_aux:
   assumes "graph_abs M"
-  assumes "wf_input \<sigma> us"
+  assumes "arriving_U us \<inter> set \<sigma> = {}"
   shows "graph_abs (ranking_aux \<sigma> us M)"
   using assms
-  by (induction us arbitrary: M) (auto simp: wf_input_def graph_abs_step)
+  by (induction us arbitrary: M) (auto simp: graph_abs_step)
 
 
-lemma wf_input_matching_ranking_aux:
+lemma matching_ranking_aux:
   assumes "graph_abs M"
   assumes "matching M"
-  assumes "wf_input \<sigma> us"
+  assumes "arriving_U us \<inter> set \<sigma> = {}"
   assumes "arriving_U us \<inter> Vs M = {}"
+  assumes "distinct (map fst us)"
   shows "matching (ranking_aux \<sigma> us M)"
   using assms
 proof (induction \<sigma> us M rule: ranking_aux.induct)
   case (2 \<sigma> u ns us M)
-  then have 1: "graph_abs (step \<sigma> M u ns)" "matching (step \<sigma> M u ns)" "wf_input \<sigma> us"
-    by (auto intro: graph_abs_step matching_step dest: wf_input_hd wf_input_tl)
+  then have 1: "graph_abs (step \<sigma> M u ns)" "matching (step \<sigma> M u ns)"
+    by (auto intro: graph_abs_step matching_step)
+
   have disjoint': "arriving_U us \<inter> ({u} \<union> set \<sigma> \<union> Vs M) = {}"
     using "2.prems"
-    unfolding wf_input_def
     by (simp add: Int_Un_distrib Int_commute)
 
   then have "arriving_U us \<inter> Vs (step \<sigma> M u ns) = {}"
     by (smt (z3) Int_Un_distrib disjoint_iff insertCI sup_bot.neutr_eq_iff vs_step)
 
   then show ?case
-    using "2.IH" 1
-    by simp
+    using 2 1
+    by auto
 qed auto
 
-lemma wf_input_partitioned_bipartite_ranking_aux:
-  assumes "wf_input \<sigma> us"
+lemma partitioned_bipartite_ranking_aux:
+  assumes "arriving_U us \<inter> set \<sigma> = {}"
   assumes "partitioned_bipartite M (set \<sigma>)"
   shows "partitioned_bipartite (ranking_aux \<sigma> us M) (set \<sigma>)"
   using assms
@@ -290,78 +373,57 @@ lemma wf_input_ranking_inv_ranking_aux:
   assumes "ranking_inv \<sigma> [] M"
   shows "ranking_inv \<sigma> us (ranking_aux \<sigma> us M)"
   using assms
-  apply (auto intro!: ranking_invI wf_input_matching_ranking_aux wf_input_partitioned_bipartite_ranking_aux 
+  apply (auto intro!: ranking_invI matching_ranking_aux partitioned_bipartite_ranking_aux 
         dest: ranking_invD partitioned_bipartite_graph_absD wf_input_tl)
-  apply (metis empty_iff empty_set image_empty partitioned_bipartiteE ranking_inv_def subsetD vs_member)
-  apply (drule vs_ranking_aux)
-  apply auto
-  using ranking_inv_subset_\<sigma> apply fastforce
-  by (meson in_mono vs_offline_graph wf_input_def)
+      apply (metis (no_types, hide_lams) disjoint_iff fst_conv image_iff wf_input_def)
+     apply (metis (no_types, lifting) ex_in_conv imageE list.set(1) partitioned_bipartiteE ranking_invD(3) ranking_invD(4) subset_iff vs_member)
+  using wf_input_def apply blast
+   apply (metis disjoint_iff eq_fst_iff image_eqI wf_input_def)
+  by (metis (no_types, lifting) DiffI empty_iff empty_set image_empty ranking_inv_subset_\<sigma> subset_eq vs_offline_graph vs_ranking_aux wf_input_def)
 
-
-lemma wf_input_graph_abs_ranking:
-  assumes "wf_input \<sigma> us"
+lemma graph_abs_ranking:
+  assumes "arriving_U us \<inter> set \<sigma> = {}"
   shows "graph_abs (ranking \<sigma> us)"
-  by (simp add: assms ranking_PI wf_input_graph_abs_ranking_aux)
+  by (simp add: assms ranking_PI graph_abs_ranking_aux)
 
-lemma wf_input_matching_ranking:
-  assumes "wf_input \<sigma> us"
+lemma matching_ranking:
+  assumes "arriving_U us \<inter> set \<sigma> = {}"
+  assumes "arriving_U us \<inter> Vs M = {}"
+  assumes "distinct (map fst us)"
   shows "matching (ranking \<sigma> us)"
   using assms
-  by (simp add: ranking_def wf_input_matching_ranking_aux)
+  by (simp add: ranking_def matching_ranking_aux)
 
 
-lemma wf_input_graph_abs_offline_graph:
+lemma partitioned_bipartite_ranking:
+  assumes "arriving_U us \<inter> set \<sigma> = {}"
+  shows "partitioned_bipartite (ranking \<sigma> us) (set \<sigma>)"
+  using assms
+  by (simp add: ranking_def partitioned_bipartite_ranking_aux)
+
+
+lemma graph_abs_offline_graph:
   assumes "wf_input \<sigma> us"
   shows "graph_abs (offline_graph us)"
   using assms
   by (induction us rule: offline_graph.induct) 
      (auto dest: wf_input_tl wf_input_hd intro: graph_abs_union graph_abs_compr)
 
-lemma wf_input_partitioned_bipartite_offline_graph:
+lemma partitioned_bipartite_offline_graph:
   assumes "wf_input \<sigma> us"
   shows "partitioned_bipartite (offline_graph us) (set \<sigma>)"
   using assms
 proof (induction us rule: offline_graph.induct)
   case (2 u ns us)
   show ?case 
-  proof (intro partitioned_bipartiteI)
-    show "graph_abs (offline_graph ((u, ns) # us))"
-      using 2 wf_input_graph_abs_offline_graph by blast
-    show "\<And>e. e \<in> offline_graph ((u, ns) # us) \<Longrightarrow> \<exists>u' v. e = {u', v} \<and> u' \<in> set \<sigma> \<and> v \<in> Vs (offline_graph ((u, ns) # us)) - set \<sigma>"
-    proof -
-      fix e
-      assume "e \<in> offline_graph ((u, ns) # us)"
-      then have "e \<in> offline_graph us \<or> e \<in> {{u, v}| v. v \<in> ns}" by auto
-      then consider (ind) "e \<in> offline_graph us" | (new) "e \<in> {{u, v}| v. v \<in> ns}" by blast
-      then show "\<exists>u' v. e = {u', v} \<and> u' \<in> set \<sigma> \<and> v \<in> Vs (offline_graph ((u, ns) # us)) - set \<sigma>" 
-      proof cases
-        case ind
-        then show ?thesis
-          by (smt (verit) "2.IH" "2.prems" DiffD2 DiffI \<open>e \<in> offline_graph ((u, ns) # us)\<close> edges_are_Vs insert_commute partitioned_bipartiteE wf_input_tl)
-      next
-        case new
-        then obtain v where "v \<in> ns" "e = {u,v}" by blast
-        then have "v \<in> set \<sigma>" "u \<notin> set \<sigma>"
-          using 2
-          by (auto dest: wf_input_hd)
-        have "u \<in> Vs (offline_graph ((u, ns) # us))"
-          by (metis \<open>e = {u, v}\<close> \<open>e \<in> offline_graph ((u, ns) # us)\<close> edges_are_Vs)
-        then show ?thesis
-          using \<open>e = {u, v}\<close> \<open>u \<notin> set \<sigma>\<close> \<open>v \<in> set \<sigma>\<close> by blast
-      qed
-    qed
+  proof (simp, intro partitioned_bipartite_union)
+    show "partitioned_bipartite {{u,v} |v. v \<in> ns} (set \<sigma>)" using "2.prems"
+      by (auto dest: wf_input_hd intro: partitioned_bipartite_compr)
+  next
+    show "partitioned_bipartite (offline_graph us) (set \<sigma>)" using 2
+      by (auto dest: wf_input_tl)
   qed
 qed auto
-
-  
-
-lemma in_step_elim:
-  assumes "e \<in> step \<sigma> M u ns"
-  assumes "e \<notin> M"
-  obtains v where "e = {u,v}" "v \<in> ns" "v \<in> set \<sigma>" "v \<notin> Vs M"
-  using assms edge_in_step
-  by force
 
 
 lemma ranking_aux_subset_offline_graph:
@@ -381,7 +443,7 @@ lemma step_lowest_rank:
   assumes "w \<in> set \<sigma>" "w \<in> ns" "w \<notin> Vs M" "w \<noteq> v"
   assumes "{u,v} \<in> step \<sigma> M u ns"
   shows "rank \<sigma> v < rank \<sigma> w"
-  using assms
+  using assms 
   apply (induction \<sigma>)
    apply simp_all
   by (metis doubleton_eq_iff insert_iff vs_member)
@@ -393,8 +455,10 @@ lemma neighbors_of_Cons:
   using assms
   by (induction us) auto
 
+
 lemma ranking_aux_hd_ineq:
-  assumes "wf_input \<sigma> ((u', ns) # us)"
+  assumes "distinct (map fst ((u',ns)#us))"
+  assumes "set \<sigma> \<inter> arriving_U us = {}"
   assumes "v \<in> set \<sigma>"
   assumes "u \<notin> Vs (step \<sigma> M u' ns)"
   assumes "{u, v} \<in> ranking_aux \<sigma> ((u', ns) # us) M"
@@ -404,20 +468,21 @@ proof (rule ccontr, simp)
   have "u \<notin> Vs M" using assms
     by (meson step_mono vs_transport)
   have "u \<notin> arriving_U us"
-    by (metis (no_types, hide_lams) \<open>u = u'\<close> assms(1) distinct.simps(2) fst_conv list.simps(9) set_map wf_input_def)
+    by (metis (no_types, hide_lams) \<open>u = u'\<close> assms(1) distinct.simps(2) fst_conv list.simps(9) set_map)
   show False
-    by (metis (no_types, lifting) \<open>u = u'\<close> \<open>u \<notin> arriving_U us\<close> assms(1) assms(3) assms(4) edges_are_Vs ranking_aux.simps(2) subset_eq vs_offline_graph vs_ranking_aux wf_input_def wf_input_hd wf_input_tl)
+    by (smt (verit, del_insts) \<open>u \<notin> arriving_U us\<close> assms(2) assms(3) assms(4) assms(5) disjoint_iff doubleton_eq_iff edge_in_ranking_aux fst_conv image_iff insertCI ranking_aux.simps(2) vs_member)
 qed
 
 
 lemma u_in_ranking_aux:
-  assumes "wf_input \<sigma> us"
+  assumes "arriving_U us \<inter> set \<sigma> = {}"
   assumes "partitioned_bipartite M (set \<sigma>)"
   assumes "v \<in> set \<sigma>"
   assumes "u \<notin> Vs M"
   assumes "{u,v} \<in> ranking_aux \<sigma> us M"
-  shows "u \<notin> set \<sigma>"
-  by (metis DiffD2 assms(1) assms(2) assms(3) assms(5) doubleton_eq_iff partitioned_bipartiteE wf_input_partitioned_bipartite_ranking_aux)
+  shows "u \<in> arriving_U us - set \<sigma>"
+  using assms
+  by (auto dest!: edge_in_ranking_aux simp: doubleton_eq_iff intro!: rev_image_eqI)
 
 lemma u_in_stepE:
   assumes "u \<in> Vs (step \<sigma> M u ns)"
@@ -427,8 +492,45 @@ lemma u_in_stepE:
   using assms
   by (induction \<sigma> M u ns rule: step.induct) (auto split: if_splits)
 
+lemma step_matches_u_if_possible:
+  assumes "u \<notin> Vs M"
+  assumes "\<exists>v. v \<in> set \<sigma> \<inter> ns - Vs M"
+  shows "u \<in> Vs (step \<sigma> M u ns)"
+  using assms
+  apply (induction \<sigma> M u ns rule: step.induct)
+   apply simp_all
+  by (metis edges_are_Vs insertI1)
+
+lemma neighbors_of_eq:
+  assumes "distinct (map fst us)"
+  assumes "(u,ns) \<in> set us"
+  shows "neighbors_of u us = ns"
+  using assms
+proof (induction us rule: neighbors_of.induct)
+  case (2 u v ns' vs)
+  then show ?case 
+  proof (cases "u = v")
+    case True
+    then show ?thesis 
+      using 2
+      by (auto intro: eq_key_imp_eq_value simp: rev_image_eqI)
+  qed auto
+qed simp
+
+lemma u_in_step:
+  assumes "arriving_U us \<inter> set \<sigma> = {}"
+  assumes "arriving_U us \<inter> arriving_V us = {}"
+  assumes "distinct (map fst us)"
+  assumes "u \<notin> Vs M"
+  assumes "v \<notin> Vs M"
+  assumes "v \<in> set \<sigma> \<inter> neighbors_of u us"
+  shows "u \<in> Vs (step \<sigma> M u (neighbors_of u us))"
+  using assms
+  by (metis Diff_iff step_matches_u_if_possible)
+
 lemma vertex_in_step_edge_in_step:
-  assumes "wf_input \<sigma> ((u,ns)#us)"
+  assumes "arriving_U ((u,ns)#us) \<inter> set \<sigma> = {}"
+  assumes "distinct (map fst ((u, ns) # us))"
   assumes "partitioned_bipartite M (set \<sigma>)"
   assumes "matching M"
   assumes "arriving_U ((u,ns)#us) \<inter> Vs M = {}"
@@ -439,7 +541,7 @@ lemma vertex_in_step_edge_in_step:
   shows "{u,v} \<in> step \<sigma> M u ns"
 proof -
   have "u \<notin> set \<sigma>"
-    by (meson assms(1) wf_input_hd)
+    using assms by force
   with assms obtain v' where "u \<noteq> v'" "{u,v'} \<in> step \<sigma> M u ns" "v' \<in> ns" "v' \<in> set \<sigma>"
     by (auto elim: u_in_stepE)
   have "v' = v" 
@@ -448,17 +550,19 @@ proof -
     then have "{u,v'} \<in> ranking_aux \<sigma> ((u,ns)#us) M"
       by (simp add: \<open>{u, v'} \<in> step \<sigma> M u ns\<close> ranking_aux_mono)
     have "matching (ranking_aux \<sigma> ((u,ns)#us) M)"
-      by (meson assms(1) assms(2) assms(3) assms(4) partitioned_bipartite_graph_absD wf_input_matching_ranking_aux)
+      using assms
+      by (intro matching_ranking_aux partitioned_bipartite_graph_absD)
     then show False 
-      by (metis \<open>v' \<noteq> v\<close> \<open>{u, v'} \<in> ranking_aux \<sigma> ((u, ns) # us) M\<close> assms(8) doubleton_eq_iff insertI1 matching_unique_match)
+      by (metis \<open>v' \<noteq> v\<close> \<open>{u, v'} \<in> ranking_aux \<sigma> ((u, ns) # us) M\<close> assms(9) doubleton_eq_iff insertI1 matching_unique_match)
   qed
   then show ?thesis
     using \<open>{u, v'} \<in> step \<sigma> M u ns\<close> by auto
 qed
 
 
-lemma wf_input_arriving_U_disjoint_Cons:
-  assumes "wf_input \<sigma> ((u,ns)#us)"
+lemma arriving_U_disjoint_Cons:
+  assumes "distinct (map fst ((u,ns)#us))"
+  assumes "arriving_U ((u,ns)#us) \<inter> set \<sigma> = {}"
   assumes "arriving_U ((u,ns)#us) \<inter> Vs M = {}"
   shows "arriving_U us \<inter> Vs (step \<sigma> M u ns) = {}"
 proof (rule ccontr)
@@ -466,25 +570,26 @@ proof (rule ccontr)
   then obtain u' where "u' \<in> arriving_U us" "u' \<in> Vs (step \<sigma> M u ns)"
     by blast
   then consider "u' = u" | "u' \<in> Vs M"
-    by (metis assms(1) disjoint_iff vs_step wf_input_def wf_input_tl)
+    using assms vs_step by fastforce
   then show False
   proof cases
     case 1
     then show ?thesis
-      by (metis (no_types, hide_lams) \<open>u' \<in> arriving_U us\<close> assms(1) distinct.simps(2) fst_conv list.map(2) set_map wf_input_def)
+      using \<open>u' \<in> arriving_U us\<close> assms by auto
   next
     case 2
     then show ?thesis
-      using \<open>u' \<in> arriving_U us\<close> assms(2) by fastforce
+      using \<open>u' \<in> arriving_U us\<close> assms by fastforce
   qed
 qed
 
 lemma ranking_aux_lowest_rank:
-  assumes "wf_input \<sigma> us"
+  assumes "arriving_U us \<inter> set \<sigma> = {}"
+  assumes "distinct (map fst us)"
   assumes "u \<notin> Vs M"
   assumes "v \<in> set \<sigma>" \<comment> \<open>hence, u is the node that arrives\<close>
-  assumes "w \<in> set \<sigma>" "w \<in> neighbors_of u us" "w \<notin> Vs M" "w \<notin> Vs (ranking_aux \<sigma> us M)"
-  assumes "{u,v} \<in> ranking_aux \<sigma> us M"
+  assumes w_unmatched: "w \<in> set \<sigma>" "w \<in> neighbors_of u us" "w \<notin> Vs M" "w \<notin> Vs (ranking_aux \<sigma> us M)"
+  assumes uv_matched: "{u,v} \<in> ranking_aux \<sigma> us M"
   assumes "partitioned_bipartite M (set \<sigma>)"
   assumes "matching M"
   assumes "arriving_U us \<inter> Vs M = {}"
@@ -492,58 +597,138 @@ lemma ranking_aux_lowest_rank:
   using assms
 proof (induction \<sigma> us M rule: ranking_aux.induct)
   case (2 \<sigma> u' ns us M)
-
   have "u \<notin> set \<sigma>"
-    by (meson "2.prems"(1) "2.prems"(2) "2.prems"(3) "2.prems"(8) "2.prems"(9) u_in_ranking_aux)
+    by (meson "2.prems" DiffD2 u_in_ranking_aux)
 
   have "w \<noteq> v"
-    using assms(7) assms(8) insert_commute by auto
+    using uv_matched insert_commute w_unmatched(4) by blast
 
   consider (ind) "u \<notin> Vs (step \<sigma> M u' ns)" | (new) "u \<in> Vs (step \<sigma> M u' ns)" by blast
   then show ?case
   proof cases
     case ind
     have "w \<in> set \<sigma>" 
-      using "2.prems"(4) by blast
-    have "w \<in> neighbors_of u us"
-      apply (rule neighbors_of_Cons[where u' = u'])
-       apply (metis "2.prems"(1) "2.prems"(3) "2.prems"(8) ind ranking_aux_hd_ineq wf_input_hd)
-      using "2.prems"(5) by blast
+      using "2.prems" by blast
+
+    have "u \<noteq> u'"
+      using "2.prems"(1) "2.prems"(2) "2.prems"(4) "2.prems"(9) ind ranking_aux_hd_ineq by fastforce
+
+     have "w \<in> neighbors_of u us"
+       by (rule neighbors_of_Cons[OF \<open>u \<noteq> u'\<close> "2.prems"(6)])
+
     have "w \<notin> Vs (step \<sigma> M u' ns)"
-      by (metis "2.prems"(7) ranking_aux.simps(2) ranking_aux_mono vs_member_elim vs_member_intro)
+      by (metis (full_types) "2"(9) ranking_aux.simps(2) ranking_aux_mono vs_transport)
+
     have "arriving_U us \<inter> Vs (step \<sigma> M u' ns) = {}"
-      by (meson "2.prems"(1) "2.prems"(11) wf_input_arriving_U_disjoint_Cons)
+      by (meson "2.prems" arriving_U_disjoint_Cons)
+
     show ?thesis
       apply (rule "2.IH")
-      using "2.prems"(1) wf_input_tl apply blast
+      using "2.prems"(1) apply simp
       apply (simp_all add: "2.prems" ind \<open>w \<in> neighbors_of u us\<close> \<open>w \<notin> Vs (step \<sigma> M u' ns)\<close> \<open>arriving_U us \<inter> Vs (step \<sigma> M u' ns) = {}\<close>)
-      using "2.prems"(7) apply force
+      using "2.prems"(2) apply force
       using "2.prems"(8) apply force
-        apply (meson "2.prems"(1) "2.prems"(9) partitioned_bipartite_step wf_input_hd)
-       apply (metis "2.prems"(1) "2.prems"(10) "2.prems"(11) disjoint_iff fst_conv image_eqI list.set_intros(1) matching_step wf_input_hd)
+      using "2.prems"(9) apply auto[1]
+       apply (metis "2.prems"(1) "2.prems"(10) disjoint_iff fst_conv image_eqI list.set_intros(1) partitioned_bipartite_step)
+      using "2.prems"(1) "2.prems"(11) "2.prems"(12) matching_step apply fastforce
       done
   next
     case new
     have "u' = u"
-      by (metis "2.prems"(2) \<open>u \<notin> set \<sigma>\<close> new vs_step)
+      by (metis "2.prems" \<open>u \<notin> set \<sigma>\<close> new vs_step)
     then have "{u,v} \<in> step \<sigma> M u ns"
-      by (metis "2.prems"(1) "2.prems"(10) "2.prems"(11) "2.prems"(2) "2.prems"(3) "2.prems"(8) "2.prems"(9) new vertex_in_step_edge_in_step)
+      by (metis "2.prems" new vertex_in_step_edge_in_step)
     have "w \<in> ns"
-      using "2.prems"(5) \<open>u' = u\<close> by auto
+      using "2.prems" \<open>u' = u\<close> by auto
     show ?thesis
-      by (meson "2.prems"(2) "2.prems"(4) "2.prems"(6) \<open>u \<notin> set \<sigma>\<close> \<open>w \<in> ns\<close> \<open>w \<noteq> v\<close> \<open>{u, v} \<in> step \<sigma> M u ns\<close> step_lowest_rank)
+      by (meson "2.prems" \<open>u \<notin> set \<sigma>\<close> \<open>w \<in> ns\<close> \<open>w \<noteq> v\<close> \<open>{u, v} \<in> step \<sigma> M u ns\<close> step_lowest_rank)
   qed
 qed simp
 
-
-lemma ranking_lowest_rank:
-  assumes "wf_input \<sigma> us"
+theorem ranking_lowest_rank:
+  assumes "arriving_U us \<inter> set \<sigma> = {}"
+  assumes "distinct (map fst us)"
   assumes "v \<in> set \<sigma>"
   assumes "w \<in> set \<sigma>" "w \<in> neighbors_of u us" "w \<notin> Vs (ranking \<sigma> us)"
   assumes "{u,v} \<in> ranking \<sigma> us"
   shows "rank \<sigma> v < rank \<sigma> w"
   using assms
   by (intro ranking_aux_lowest_rank[where u = u and M = "{}"]) (simp_all add: ranking_def)
+
+
+lemma ranking_aux_first_arrival:
+  assumes "arriving_U us \<inter> set \<sigma> = {}"
+  assumes "distinct (map fst us)"
+
+  assumes "v \<in> set \<sigma>" "v \<in> neighbors_of u us"
+  assumes "u \<in> arriving_U us" "u \<notin> Vs (ranking_aux \<sigma> us M)"
+  assumes "{u',v} \<in> ranking_aux \<sigma> us M"
+
+  assumes "u \<notin> Vs M" "u' \<notin> Vs M"
+  assumes "partitioned_bipartite M (set \<sigma>)"
+  assumes "matching M"
+  assumes "arriving_U us \<inter> Vs M = {}"
+
+  shows "arrival us u' < arrival us u"
+  using assms
+proof (induction \<sigma> us M rule: ranking_aux.induct)
+  case (2 \<sigma> u'' ns us M)
+
+  have "u \<noteq> u'"
+    by (metis assms edges_are_Vs)
+
+  have "v \<notin> Vs M"
+    by (smt (verit, ccfv_SIG) "2.prems" disjoint_iff doubleton_eq_iff edge_in_ranking_aux fst_conv image_eqI insertCI vs_member_intro)
+
+  have "u'' \<noteq> u"
+  proof (rule ccontr, simp only: not_not)
+    assume "u'' = u"
+    then have "neighbors_of u ((u'',ns)#us) = ns" 
+      by simp
+    then have "u \<in> Vs (step \<sigma> M u ns)"
+      apply (intro step_matches_u_if_possible)
+       apply (simp add: "2.prems")
+      by (metis "2.prems" Diff_iff IntI \<open>v \<notin> Vs M\<close> in_mono neighbors_of.simps(2) wf_input_hd)
+
+    then have "u \<in> Vs (ranking_aux \<sigma> ((u'',ns)#us) M)"
+      by (metis \<open>u'' = u\<close> ranking_aux.simps(2) ranking_aux_mono vs_member)
+    then show False using "2.prems"
+      by blast
+  qed
+
+  then consider (new) "u'' = u'" | (ind) "u'' \<noteq> u \<and> u'' \<noteq> u'" by blast
+  then show ?case 
+  proof cases
+    case new
+    then show ?thesis using \<open>u'' \<noteq> u\<close> by fastforce
+  next
+    case ind
+    then show ?thesis
+      apply (auto intro!: "2.IH"[simplified])
+      using "2.prems"(1) apply fastforce
+      using "2.prems"(2) apply auto[1]
+               apply (simp add: "2.prems")
+      using "2.prems"(4) apply force
+      using "2.prems"(5) apply auto[1]
+      using "2.prems"(6) apply fastforce
+      using "2.prems"(7) apply force
+          apply (metis "2.prems" ranking_aux.simps(2) ranking_aux_mono vs_member)
+         apply (metis "2.prems" u_in_ranking_aux vs_step)
+      using "2.prems"(1) "2.prems"(10) partitioned_bipartite_step apply fastforce
+       apply (metis "2.prems" disjoint_iff fst_conv image_iff list.set_intros(1) matching_step wf_input_hd)
+      by (smt (verit, ccfv_SIG) "2.prems" disjoint_iff distinct.simps(2) fst_conv image_iff insert_iff list.set(2) list.simps(9) set_map vs_step wf_input_def)
+  qed
+qed simp
+
+theorem ranking_first_arrival:
+  assumes "arriving_U us \<inter> set \<sigma> = {}"
+  assumes "distinct (map fst us)"
+  assumes "v \<in> set \<sigma>" "v \<in> neighbors_of u us"
+  assumes "u \<in> arriving_U us" "u \<notin> Vs (ranking \<sigma> us)"
+  assumes "{u',v} \<in> ranking \<sigma> us"
+  shows "arrival us u' < arrival us u"
+  using assms
+  by (intro ranking_aux_first_arrival[where u = u and M = "{}"]) (simp_all add: ranking_def)
 
 
 definition move_to :: "'a list \<Rightarrow> 'a \<Rightarrow> nat \<Rightarrow> 'a list" ("_ \<mapsto>\<index> _" [100,100] 40) where 
@@ -556,6 +741,11 @@ lemma move_to_gt_length:
   "length xs \<le> i \<Longrightarrow> (v \<mapsto>\<^bsub>xs\<^esub> i) = (v \<mapsto>\<^bsub>xs\<^esub> length xs)"
   unfolding move_to_def
   by (auto intro!: append_cong dest: le_trans[OF length_filter_le])
+
+lemma move_to_set: "set (x \<mapsto>\<^bsub>xs\<^esub> i) = set xs \<union> {x}"
+  unfolding move_to_def
+  apply (auto dest: in_set_takeD in_set_dropD)
+  by (metis (mono_tags, lifting) append_take_drop_id filter_set last_index_append last_index_size_conv length_append member_filter)
 
 lemma move_to_Cons_Suc:
   assumes "x \<noteq> v"
@@ -592,6 +782,14 @@ lemma move_to_distinct:
   "distinct xs \<Longrightarrow> distinct (x \<mapsto>\<^bsub>xs\<^esub> i)"
   unfolding move_to_def
   by (auto dest: in_set_dropD in_set_takeD distinct_filter set_take_disj_set_drop_if_distinct)
+
+lemma wf_input_move_to:
+  assumes "wf_input \<sigma> us"
+  assumes "v \<in> set \<sigma>"
+  shows "wf_input (v \<mapsto>\<^bsub>\<sigma>\<^esub> i) us"
+  using assms
+  unfolding wf_input_def
+  by (auto simp: move_to_set move_to_distinct)
 
 
 lemma induct_list_nat[case_names nil_zero nil_suc cons_zero cons_suc]:
@@ -648,7 +846,7 @@ lemma not_Nil_length_SucE: "xs \<noteq> [] \<Longrightarrow> (\<And>n. length xs
 
 
 lemma move_to_id:
-  "count_list \<sigma> v = 1 \<Longrightarrow> (v \<mapsto>\<^bsub>\<sigma>\<^esub> (rank \<sigma> v)) = \<sigma>"
+  "count_list \<sigma> v = (Suc 0) \<Longrightarrow> (v \<mapsto>\<^bsub>\<sigma>\<^esub> (rank \<sigma> v)) = \<sigma>"
   by (induction \<sigma>) (auto simp: move_to_0 filter_id_conv move_to_Cons_Suc count_zero)
 
 lemma move_to_front_less:
@@ -725,6 +923,9 @@ lemma move_to_back_gr:
 lemma distinct_count_list_le: "distinct xs \<Longrightarrow> count_list xs x \<le> 1"
   by (induction xs) auto
 
+lemma distinct_count_in_set: "distinct xs \<Longrightarrow> x \<in> set xs \<Longrightarrow> count_list xs x = 1"
+  by (induction xs) auto
+
 
 lemma move_to_rank_v:
   assumes "distinct \<sigma>"
@@ -753,6 +954,368 @@ proof (induction \<sigma> i rule: induct_list_nat)
              dest: in_set_takeD index_take_if_set  split: if_splits)
 qed auto
 
+lemma
+  assumes "distinct xs"
+  assumes "xs = ps @ x # ss"
+  assumes "i \<le> rank xs x"
+  obtains pps pss where "(x \<mapsto>\<^bsub>xs\<^esub> i) = pps @ x # pss @ ss" "pps @ pss = ps"
+  using assms
+proof (induction xs i arbitrary: ps rule: induct_list_nat)
+  case (cons_zero a xs)
+  then show ?case
+    by (auto simp: move_to_0 not_in_set_filter_id) blast
+next
+  case (cons_suc a xs n)
+  consider (eq) "a = x" | (neq) "a \<noteq> x" by blast
+  then show ?case
+  proof cases
+    case eq
+    with cons_suc.prems have "ps = []" 
+      by (auto simp: Cons_eq_append_conv)
+    with cons_suc show ?thesis 
+      by (auto simp: move_to_0 not_in_set_filter_id)
+  next
+    case neq
+
+    with cons_suc.prems obtain tl_ps where "ps = a # tl_ps" 
+      by (auto simp: Cons_eq_append_conv)
+
+    with cons_suc.prems have "xs = tl_ps @ x # ss" 
+      by simp
+
+    have "distinct xs"
+      using cons_suc.prems(2) by simp
+
+    have "n \<le> rank xs x" 
+      using cons_suc.prems(4) neq by auto
+
+    then obtain pps pss where "(x \<mapsto>\<^bsub>xs\<^esub> n) = pps @ x # pss @ ss" "pps @ pss = tl_ps"
+      thm cons_suc.IH
+      sorry
+
+    then show ?thesis sorry
+  qed
+qed auto
+
+lemma step_append:
+  "u \<notin> Vs M \<Longrightarrow> step (\<sigma> @ \<sigma>') M u ns = (if u \<in> Vs (step \<sigma> M u ns) then step \<sigma> M u ns else step \<sigma>' M u ns)"
+  by (induction \<sigma> M u ns rule: step.induct) (simp_all add: Vs_def, fastforce)
+
+lemma step_no_change:
+  assumes "set \<sigma> \<inter> ns - Vs M = {}"
+  shows "step \<sigma> M u ns = M"
+  using assms 
+  by (induction \<sigma> M u ns rule: step.induct) auto
+
+lemma ranking_aux_append_vs:
+  assumes "arriving_U us \<inter> set (\<sigma> @ \<sigma>') = {}"
+  assumes "arriving_U us \<inter> arriving_V us = {}"
+  assumes "distinct (map fst us)"
+  assumes "arriving_U us \<inter> Vs M = {}"
+  shows "ranking_aux (\<sigma> @ \<sigma>') us M = ranking_aux \<sigma>' [u <- us. fst u \<notin> Vs (ranking_aux \<sigma> us M)] (ranking_aux \<sigma> us M)"
+  using assms
+proof (induction us arbitrary: M)
+  case (Cons a us)
+  obtain u ns where a_pair: "a = (u,ns)" by fastforce
+  then have "u \<notin> Vs M"
+    using Cons.prems by fastforce
+
+  have disjoint_step: "arriving_U us \<inter> Vs (step \<sigma> M u ns) = {}" 
+    using Cons.prems
+    unfolding a_pair
+    by (simp add: Int_Un_distrib arriving_U_disjoint_Cons bot_eq_sup_iff)
+
+  have disjoint_step': "arriving_U us \<inter> Vs (step (\<sigma> @ \<sigma>') M u ns) = {}"
+    using Cons.prems
+    unfolding a_pair
+    by (simp add: Int_Un_distrib arriving_U_disjoint_Cons bot_eq_sup_iff)
+
+  have neighbors: "neighbors_of u ((u,ns)#us) = ns" by simp
+
+  have p1: "arriving_U us \<inter> set (\<sigma> @ \<sigma>') = {}"
+    using Cons.prems(1) by force
+  have p2: "arriving_U us \<inter> arriving_V us = {}"
+    using Cons.prems(2) UnCI by fastforce
+  have p3: "distinct (map fst us)" using Cons.prems by simp
+
+  let ?r_pref = "(ranking_aux \<sigma> ((u,ns)#us) M)" and ?r_full = "(ranking_aux (\<sigma> @ \<sigma>') ((u,ns)#us) M)"
+
+  consider (matched_prefix) "u \<in> Vs ?r_pref" | (matched_suffix) "u \<notin> Vs ?r_pref \<and> u \<in> Vs ?r_full" | 
+    (not_matched) "u \<notin> Vs ?r_pref \<and> u \<notin> Vs ?r_full" by blast
+
+  then show ?case 
+  proof cases
+    case matched_prefix
+    then obtain v where "{u,v} \<in> ranking_aux \<sigma> ((u,ns)#us) M" "v \<notin> Vs M" "v \<in> ns \<inter> set \<sigma>"
+      by (smt (verit, del_insts) Cons.prems(1) Cons.prems(3) IntE Int_Un_distrib \<open>u \<notin> Vs M\<close> a_pair distinct.simps(2) edge_in_ranking_aux fst_conv image_eqI insert_disjoint(1) insert_iff list.simps(15) list.simps(9) set_append set_map snd_conv sup_bot.neutr_eq_iff vs_member)
+  
+    have "u \<in> Vs (step \<sigma> M u ns)"
+      apply (subst neighbors[symmetric])
+      apply (rule u_in_step[where v=v])
+           apply (metis Cons.prems(1) Int_Un_distrib a_pair set_append sup_bot.neutr_eq_iff)
+      using Cons.prems(2) a_pair apply fastforce
+      using Cons.prems(3) a_pair apply blast
+        apply (simp add: \<open>u \<notin> Vs M\<close>)
+       apply (simp add: \<open>v \<notin> Vs M\<close>)
+      using \<open>v \<in> ns \<inter> set \<sigma>\<close> by auto
+
+    with \<open>u \<notin> Vs M\<close> have step_append_eq: "step (\<sigma> @ \<sigma>') M u ns = step \<sigma> M u ns" by (simp add: step_append)
+
+    with matched_prefix Cons.IH[OF p1 p2 p3 disjoint_step] show ?thesis
+      by (auto simp: a_pair)
+  next
+    case matched_suffix
+    then show ?thesis sorry
+  next
+    case not_matched
+    then have "u \<notin> Vs (step \<sigma> M u ns)"
+      by (metis (full_types) ranking_aux.simps(2) ranking_aux_mono vs_transport)
+
+    then have step_M: "step \<sigma> M u ns = M"
+      by (metis \<open>u \<notin> Vs M\<close> append_Nil2 step.simps(1) step_append)
+
+    with \<open>u \<notin> Vs M\<close> have step_append_eq: "step (\<sigma> @ \<sigma>') M u ns = step \<sigma>' M u ns" by (simp add: step_append)
+
+    from not_matched have "u \<notin> Vs (step \<sigma>' M u ns)"
+      by (metis (full_types) ranking_aux.simps(2) ranking_aux_mono step_append_eq vs_transport)
+
+    then have step'_M: "step \<sigma>' M u ns = M"
+      by (metis \<open>u \<notin> Vs M\<close> append_Nil2 step.simps(1) step_append)
+
+    have "u \<notin> Vs (ranking_aux \<sigma> us M)"
+      using not_matched step_M by force
+
+    have "u \<notin> Vs (step \<sigma>' (ranking_aux \<sigma> us M) u ns)"
+    proof (rule ccontr, simp)
+      assume "u \<in> Vs (step \<sigma>' (ranking_aux \<sigma> us M) u ns)"
+      then have "u \<in> Vs (ranking_aux \<sigma>' ((u,ns)#us) (ranking_aux \<sigma> us M))"
+        by (metis (full_types) ranking_aux.simps(2) ranking_aux_mono vs_transport)
+
+      then have "u \<in> Vs (ranking_aux \<sigma>' ((u,ns)#us) M)" sorry
+
+      then have "u \<in> Vs (ranking_aux (\<sigma> @ \<sigma>') ((u,ns)#us) M)" sorry
+      then show False
+        using not_matched by blast
+    qed
+
+    then have step'_ranking_aux: "step \<sigma>' (ranking_aux \<sigma> us M) u ns = ranking_aux \<sigma> us M" 
+      apply (intro step_no_change)
+    proof (rule ccontr)
+      assume "u \<notin> Vs (step \<sigma>' (ranking_aux \<sigma> us M) u ns)" "set \<sigma>' \<inter> ns - Vs (ranking_aux \<sigma> us M) \<noteq> {}"
+      then obtain v where "v \<in> set \<sigma>'" "v \<in> ns" "v \<notin> Vs (ranking_aux \<sigma> us M)" by blast
+      then have "u \<in> Vs (step \<sigma>' (ranking_aux \<sigma> us M) u ns)"
+        by (meson \<open>set \<sigma>' \<inter> ns - Vs (ranking_aux \<sigma> us M) \<noteq> {}\<close> \<open>u \<notin> Vs (ranking_aux \<sigma> us M)\<close> equals0I step_matches_u_if_possible)
+      then show False
+        using \<open>u \<notin> Vs (step \<sigma>' (ranking_aux \<sigma> us M) u ns)\<close> by linarith
+    qed
+      
+
+    from not_matched Cons.IH[OF p1 p2 p3 disjoint_step] show ?thesis
+      apply (simp add: a_pair step_M step'_M step_append_eq)
+      sorry
+  qed
+qed simp
+  
+
+lemma
+  assumes "wf_input (\<sigma> @ \<sigma>') us"
+  assumes "v \<in> set \<sigma>"
+  assumes "{u,v} \<in> ranking \<sigma> us"
+  shows "{u,v} \<in> ranking (\<sigma> @ \<sigma>') us"
+  sorry
+
+
+theorem
+  assumes wf_input: "wf_input \<sigma> us"
+  assumes v_in_set: "v \<in> set \<sigma>"
+  assumes w_in_set: "w \<in> set \<sigma>" 
+  assumes w_neighbor: "w \<in> neighbors_of u us" 
+  assumes w_unmatched: "w \<notin> Vs (ranking \<sigma> us)"
+  assumes u_v_match: "{u,v} \<in> ranking \<sigma> us"
+  assumes i_less: "i < length \<sigma>"
+  assumes v'_match: "{u,v'} \<in> ranking (w \<mapsto>\<^bsub>\<sigma>\<^esub> i) us" \<comment> \<open>this assumption needs to be proven\<close>
+  shows "rank (w \<mapsto>\<^bsub>\<sigma>\<^esub> i) v' \<le> rank \<sigma> w"
+proof -
+  let ?\<sigma>i = "(w \<mapsto>\<^bsub>\<sigma>\<^esub> i)"
+
+  have set_move_to: "set ?\<sigma>i = set \<sigma>" using w_in_set by (auto simp: move_to_set)
+
+  have partitioned_bipartite: "partitioned_bipartite (ranking \<sigma> us) (set \<sigma>)"
+    using wf_input
+    by (simp add: wf_input_partitioned_bipartite_ranking)
+
+  then have u_in_U: "u \<notin> set \<sigma>"
+    using u_v_match v_in_set
+    by (auto elim: partitioned_bipartiteE)
+
+  have v_once: "count_list \<sigma> v = 1"
+    using wf_input v_in_set
+    by (auto dest!: wf_input_distinctD distinct_count_in_set)
+
+  have wf_input_move_to: "wf_input ?\<sigma>i us" 
+    using wf_input_move_to[OF wf_input w_in_set]
+    by blast
+
+  have matching_move_to: "matching (ranking ?\<sigma>i us)"
+    by (simp add: wf_input_move_to wf_input_matching_ranking)
+
+  have partitioned_bipartite_move_to: "partitioned_bipartite (ranking ?\<sigma>i us) (set \<sigma>)"
+    using wf_input_move_to
+    by (simp add: wf_input_move_to wf_input_partitioned_bipartite_ranking flip: set_move_to)
+
+
+  have w_in_move: "w \<in> set ?\<sigma>i" by (auto simp: move_to_set)
+  have w_rank_i: "rank ?\<sigma>i w = i" 
+    using move_to_rank_v wf_input i_less
+    by (force dest: wf_input_distinctD)
+
+  have v'_in_set: "v' \<in> set \<sigma>"
+    using partitioned_bipartite_move_to u_in_U v'_match
+    by (auto elim: partitioned_bipartiteE)
+
+  have rank_v_less_rank_w: "rank \<sigma> v < rank \<sigma> w" 
+    using assms ranking_lowest_rank
+    by metis
+
+  consider (match_w) "rank ?\<sigma>i w \<le> rank \<sigma> v" | (match_v) "rank \<sigma> v < rank ?\<sigma>i w" by linarith
+  then show ?thesis
+  proof cases
+    case match_w
+    have w_match: "v' = w" \<comment> \<open>This is not necessarily true, i.e. when w is matched to some u' before u arrives. The cascading also takes effect here.\<close>
+    proof (rule ccontr)
+      assume "v' \<noteq> w"
+      have "rank ?\<sigma>i v' < rank ?\<sigma>i w" 
+        apply (rule ranking_lowest_rank[where u=u and us=us])
+             apply (simp add: wf_input_move_to)
+            apply (simp_all add: set_move_to v'_in_set w_in_set w_neighbor)
+        sorry
+      show False sorry
+    qed
+    then show ?thesis
+      using rank_v_less_rank_w w_rank_i match_w by simp
+  next
+    case match_v
+    have "w \<notin> Vs (ranking ?\<sigma>i us)" sorry
+    have v_match: "v' = v"
+    proof (rule ccontr)
+      assume "v' \<noteq> v"
+      have "rank ?\<sigma>i v' < rank ?\<sigma>i v"
+        apply (rule ranking_lowest_rank[where u=u and us = us])
+        sorry
+      show False sorry
+    qed
+    then show ?thesis sorry
+  qed
+qed
+
+lemma step_filter_offline_eq:
+  assumes "x \<notin> Vs (step \<sigma> M u ns)"
+  shows "step [v <- \<sigma>. v \<noteq> x] M u ns = step \<sigma> M u ns"
+  using assms
+proof (induction \<sigma> M u ns rule: step.induct)
+  case (2 v vs M u neighbors)
+  then show ?case
+    by (smt (verit, del_insts) edges_are_Vs filter.simps(2) insertCI insert_commute step.simps(2))
+qed simp
+
+lemma step_filter_online_eq:
+  assumes "x \<notin> Vs (step \<sigma> M x ns)"
+  shows "step \<sigma> M x ns = M"
+  using assms
+proof (induction \<sigma> M x ns rule: step.induct)
+  case (2 v vs M u neighbors)
+  then show ?case
+    by (metis insertI1 step.simps(2) vs_member)
+qed simp
+
+lemma step_filter_online_neighbors_eq:
+  assumes "x \<notin> Vs (step \<sigma> M u ns)"
+  shows "step \<sigma> M u (ns - {x}) = step \<sigma> M u ns"
+  using assms
+proof (induction \<sigma> M u ns rule: step.induct)
+  case (2 v vs M u neighbors)
+  then show ?case
+    by (smt (verit, ccfv_threshold) DiffE DiffI insertI1 insert_commute singletonD step.simps(2) vs_member)
+qed simp
+  
+
+lemma ranking_aux_filter_offline_eq:
+  assumes "x \<notin> Vs (ranking_aux \<sigma> us M)"
+  shows "ranking_aux [v <- \<sigma>. v \<noteq> x] us M = ranking_aux \<sigma> us M"
+  using assms
+proof (induction \<sigma> us M rule: ranking_aux.induct)
+  case (2 \<sigma> u ns us M)
+  then have "x \<notin> Vs (step \<sigma> M u ns)"
+    by (metis ranking_aux.simps(2) ranking_aux_mono vs_member)
+  from step_filter_offline_eq[OF this] have "step [v <- \<sigma>. v \<noteq> x] M u ns = step \<sigma> M u ns" by simp
+  with 2 show ?case 
+    by simp
+qed simp
+
+lemma ranking_aux_filter_online_eq:
+  assumes "x \<notin> Vs (ranking_aux \<sigma> us M)"
+  shows "ranking_aux \<sigma> [(u,ns) <- us. u \<noteq> x] M = ranking_aux \<sigma> us M"
+  using assms
+proof (induction \<sigma> us M rule: ranking_aux.induct)
+  case (2 \<sigma> u ns us M)
+  then have x_not_in_step: "x \<notin> Vs (step \<sigma> M u ns)"
+    by (metis ranking_aux.simps(2) ranking_aux_mono vs_member)
+  then show ?case
+  proof (cases "u = x")
+    case True
+    with x_not_in_step have "step \<sigma> M u ns = M"
+      by (metis step_filter_online_eq)
+    with 2 show ?thesis by simp
+  next
+    case False
+    with 2 show ?thesis by simp
+  qed
+qed simp
+
+lemma ranking_aux_filter_online_neighbors_eq:
+  assumes "x \<notin> Vs (ranking_aux \<sigma> us M)"
+  shows "ranking_aux \<sigma> (map (\<lambda>(u,ns). (u, ns - {x})) us) M = ranking_aux \<sigma> us M"
+  using assms
+proof (induction \<sigma> us M rule: ranking_aux.induct)
+  case (2 \<sigma> u ns us M)
+  then have "x \<notin> Vs (step \<sigma> M u ns)" 
+    by (metis ranking_aux.simps(2) ranking_aux_mono vs_member)
+  from step_filter_online_neighbors_eq[OF this] have "step \<sigma> M u (ns - {x}) = step \<sigma> M u ns" by simp
+  with 2 show ?case 
+    by simp
+qed simp
+
+lemma ranking_filter_offline_eq:
+  assumes "x \<notin> Vs (ranking \<sigma> us)"
+  shows "ranking [v <- \<sigma>. v \<noteq> x] us = ranking \<sigma> us"
+  using assms
+  by (simp add: ranking_def ranking_aux_filter_offline_eq)
+
+lemma ranking_filter_online_eq:
+  assumes "x \<notin> Vs (ranking \<sigma> us)"
+  shows "ranking \<sigma> [(u,ns) <- us. u \<noteq> x] = ranking \<sigma> us"
+  using assms
+  by (simp add: ranking_def ranking_aux_filter_online_eq)
+
+lemma ranking_filter_online_neighbors_eq:
+  assumes "x \<notin> Vs (ranking \<sigma> us)"
+  shows "ranking \<sigma> (map (\<lambda>(u,ns). (u, ns - {x})) us) = ranking \<sigma> us"
+  using assms
+  by (simp add: ranking_def ranking_aux_filter_online_neighbors_eq)
+
+lemma ranking_remove_vertex_eq:
+  assumes "x \<notin> Vs (ranking \<sigma> us)"
+  shows "ranking [v <- \<sigma>. v \<noteq> x] [(u,ns) <- (map (\<lambda>(u,ns). (u, ns - {x})) us). u \<noteq> x] = ranking \<sigma> us"
+  using assms
+  by (simp add: ranking_filter_offline_eq ranking_filter_online_eq ranking_filter_online_neighbors_eq)
+
+
+inductive remove_vertex_path :: "'a \<Rightarrow> 'a list \<Rightarrow> ('a \<times> 'a set) list \<Rightarrow> 'a graph \<Rightarrow> 'a list \<Rightarrow> bool" where
+  unmatched:  "x \<notin> Vs M \<Longrightarrow> remove_vertex_path x \<sigma> us M []"
+| matched_boy: "{u,x} \<in> M \<Longrightarrow> x \<in> set \<sigma> \<Longrightarrow> u \<in> arriving_U us \<Longrightarrow> remove_vertex_path u \<sigma> us M vs \<Longrightarrow> remove_vertex_path x \<sigma> us M (x#vs)"
+| matched_girl: "x \<in> set \<sigma> \<Longrightarrow> u \<in> arriving_U us \<Longrightarrow> {u,x} \<in> offline_graph us 
+  \<Longrightarrow> (\<And>x'. x' \<in> set \<sigma>  \<Longrightarrow> rank \<sigma> x' < rank \<sigma> x \<Longrightarrow> {u,x'} \<notin> offline_graph us \<or> (\<exists>u' \<in> arriving_U us. arrival us u' < arrival us u \<and> {u',x'} \<in> M))
+  \<Longrightarrow> remove_vertex_path x \<sigma> us M vs \<Longrightarrow> remove_vertex_path u \<sigma> us M (x#vs)"
 
 
 end
